src/QuerySemantic.v
@@ -26,6 +26,12 @@ Require Import Ssromega.
 
 Require Import SeqExtra.
 
+Require Import ValidFragments.
+Require Import QueryRewrite.
+
+Require Import NRGTNF.
+
+
 Section QuerySemantic.
 
   Variables N Name Vals : ordType.
@@ -36,166 +42,14 @@ Section QuerySemantic.
   Ltac apply_and3P := apply/and3P; split=> //.
   
   Variable s : @wfSchema Name Vals.
-
-  Definition does_fragment_type_apply object_type fragment_type :=
-    if is_object_type s fragment_type then
-      object_type == fragment_type
-    else
-      if is_interface_type s fragment_type then
-        object_type \in implementation s fragment_type
-      else
-        if is_union_type s fragment_type then
-          object_type \in union_members s fragment_type
-        else
-          false .
-
-  Equations? ble (label : Name) (object_type : @NamedType Name) (queries : seq (@Query Name Vals)) (p : Name -> Name -> bool) :
-    seq (@Query Name Vals) by wf (queries_size queries) :=
-    {
-      ble _ _ [::] _ := [::];
-
-      ble k O__t (InlineFragment t φ :: qs) p
-        with does_fragment_type_apply O__t t :=
-        {
-        | true := ble k O__t φ p ++ ble k O__t qs p;
-        | _ := ble k O__t qs p
-        };
-
-      ble k O__t (SingleField f α :: qs) p
-        with p f k :=
-        {
-        | true := SingleField f α :: ble k O__t qs p;
-        | _ := ble k O__t qs p
-        };
-      
-      ble k O__t (LabeledField l f α :: qs) p
-        with  p l k :=
-        {
-        | true := LabeledField l f α :: ble k O__t qs p;
-        | _ := ble k O__t qs p
-        };
-
-      
-      ble k O__t (NestedField f α φ :: qs) p
-        with p f k :=
-        {
-        | true := NestedField f α φ :: ble k O__t qs p;
-        | _ := ble k O__t qs p
-        };
-      
-      ble k O__t (NestedLabeledField l f α φ :: qs) p
-        with p l k :=
-        {
-        | true := NestedLabeledField l f α φ  :: ble k O__t qs p;
-        | _ := ble k O__t qs p
-        }
-    }.
-  all: do ?simp query_size; ssromega.
-  Qed.
-
-  Lemma ble_leq_size l O__t qs p :
-    queries_size (ble l O__t qs p) <= queries_size qs.
-  Proof.
-    funelim (ble _ _ qs _) => //=; simp query_size; rewrite ?queries_size_app; ssromega.
-  Qed.
+  Variable g : @conformedGraph Name Vals s.
   
-  
-  Definition find_queries_with_label (label : Name) (object_type : @NamedType Name) (queries : seq (@Query Name Vals)) :=
-    ble label object_type queries (fun f label => f == label).
-
-
-  Lemma found_queries_are_fields k O__t qs :
-    all (fun q => q.(is_field)) (find_queries_with_label k O__t qs).
-  Proof.
-    rewrite /find_queries_with_label.
-    funelim (ble k O__t qs (fun f label => f == label)) => //=.
-    rewrite all_cat; apply_andP.
-  Qed.
-
-  Lemma found_queries_are_fieldsP k O__t qs :
-    forall q, q \in (find_queries_with_label k O__t qs) -> q.(is_field).
-  Proof.
-      by apply/allP; apply: found_queries_are_fields.
-  Qed.
-
-
-  Lemma all_same_label label O__t qs :
-    all (fun q => match q with
-               | InlineFragment _ _ => true
-               | SingleField f _
-               | NestedField f _ _ => f == label 
-               | LabeledField l _ _
-               | NestedLabeledField l _ _ _ => l == label
-               end) (find_queries_with_label label O__t qs).
-  Proof.
-    rewrite /find_queries_with_label.
-    funelim (ble label O__t qs _) => //=; rewrite ?Heq ?andTb //.
-    rewrite all_cat; apply_andP.
-  Qed.
-
-  Lemma found_queries_leq_size l O__t qs :
-    queries_size (find_queries_with_label l O__t qs) <= queries_size qs.
-  Proof.
-      by rewrite /find_queries_with_label; apply: ble_leq_size.
-  Qed.
-
-  Hint Resolve found_queries_leq_size.
-  
-   Equations? filter_queries_with_label (label : Name) (queries : seq (@Query Name Vals)) :
-    seq (@Query Name Vals) by wf (queries_size queries) :=
-    {
-      filter_queries_with_label _ [::] := [::];
-
-      filter_queries_with_label l (InlineFragment t φ :: qs) := InlineFragment t (filter_queries_with_label l φ) :: filter_queries_with_label l qs;
-
-      filter_queries_with_label l (q :: qs)
-        with (qresponse_name q _) != l :=
-        {
-        | true := q :: filter_queries_with_label l qs;
-        | _ := filter_queries_with_label l qs
-        }     
-
-    }.
-  all: do ?[simp query_size; ssromega].
-  Qed.
-
-  Lemma filter_queries_with_label_leq_size l qs :
-    queries_size (filter_queries_with_label l qs) <= queries_size qs.
-  Proof.
-    funelim (filter_queries_with_label l qs) => //=; do ?[simp query_size; ssromega]. 
-  Qed.
-  
-    
-  Equations merge_selection_sets : seq (@Query Name Vals) -> seq (@Query Name Vals) :=
-    {
-      merge_selection_sets [::] := [::];
-      merge_selection_sets (q :: qs) := q.(qsubqueries) ++ merge_selection_sets qs
-    }.
-      
-  Lemma merged_selections_lt qs :
-    qs != [::] ->
-    queries_size (merge_selection_sets qs) < queries_size qs.
-  Proof.
-    funelim (merge_selection_sets qs) => //=.
-    case: q; intros => //=; simp query_size; rewrite ?queries_size_app;
-    case: l H => //= hd tl /(_ is_true_true) H; ssromega.
-  Qed.
-
-  Lemma merged_selections_leq qs :
-    queries_size (merge_selection_sets qs) <= queries_size qs.
-  Proof.
-    funelim (merge_selection_sets qs) => //=.
-    case: q; intros => //=; simp query_size; rewrite ?queries_size_app;
-     ssromega.
-  Qed.
-
- 
-  
-  Variable g : @graphQLGraph Name Vals.
   Implicit Type u : @node Name Vals.
   Implicit Type query : @Query Name Vals.
 
   Transparent query_size.
+
+  Reserved Notation "⟦ φ 'in' u ⟧ˢ" (at level 40).
   
   Equations? execute_selection_set u (queries : seq (@Query Name Vals)) :
     seq (Name * ResponseNode) by wf (queries_size queries) :=
@@ -203,7 +57,7 @@ Section QuerySemantic.
       execute_selection_set _ [::] := [::];
       
       execute_selection_set u (InlineFragment t φ :: qs)
-        with does_fragment_type_apply u.(type) t :=
+        with does_fragment_type_apply s u.(type) t :=
         {
         | true := execute_selection_set u (φ ++ qs);
         | _ := execute_selection_set u qs
@@ -227,14 +81,14 @@ Section QuerySemantic.
 
       
       execute_selection_set u (NestedField f α φ :: qs)
-        with lookup_field_type s u.(type) f :=
+        with lookup_field_in_type s u.(type) f :=
         {
-        | Some (ListType ty) => (f, Array [seq Object (execute_selection_set v (φ ++ merge_selection_sets (find_queries_with_label v.(type) f qs))) | v <- neighbours_with_field g u (Field f α)]) :: execute_selection_set u (filter_queries_with_label f qs);
+        | Some (Schema.Field _ _ (ListType ty)) => (f, Array [seq Object (execute_selection_set v (φ ++ merge_selection_sets (find_queries_with_label s v.(type) f qs))) | v <- neighbours_with_field g u (Field f α)]) :: execute_selection_set u (filter_queries_with_label f qs);
         
-        | Some (NT ty)
+        | Some (Schema.Field _ _ (NT ty))
             with ohead (neighbours_with_field g u (Field f α)) :=
             {
-            | Some v => (f, Object (execute_selection_set v (φ ++ merge_selection_sets (find_queries_with_label v.(type) f qs)))) :: execute_selection_set u (filter_queries_with_label f qs);
+            | Some v => (f, Object (execute_selection_set v (φ ++ merge_selection_sets (find_queries_with_label s v.(type) f qs)))) :: execute_selection_set u (filter_queries_with_label f qs);
             
             | _ =>  (f, Leaf Null) :: execute_selection_set u (filter_queries_with_label f qs)
             };
@@ -243,14 +97,14 @@ Section QuerySemantic.
         };
 
        execute_selection_set u (NestedLabeledField l f α φ :: qs)
-        with lookup_field_type s u.(type) f :=
+        with lookup_field_in_type s u.(type) f :=
         {
-        | Some (ListType ty) => (l, Array [seq Object (execute_selection_set v (φ ++ merge_selection_sets (find_queries_with_label v.(type) l qs))) | v <- neighbours_with_field g u (Field f α)]) :: execute_selection_set u (filter_queries_with_label l qs);
+        | Some (Schema.Field _ _ (ListType ty)) => (l, Array [seq Object (execute_selection_set v (φ ++ merge_selection_sets (find_queries_with_label s v.(type) l qs))) | v <- neighbours_with_field g u (Field f α)]) :: execute_selection_set u (filter_queries_with_label l qs);
         
-        | Some (NT ty)
+        | Some (Schema.Field _ _ (NT ty))
             with ohead (neighbours_with_field g u (Field f α)) :=
             {
-            | Some v => (l, Object (execute_selection_set v (φ ++ merge_selection_sets (find_queries_with_label v.(type) l qs)))) :: execute_selection_set u (filter_queries_with_label l qs);
+            | Some v => (l, Object (execute_selection_set v (φ ++ merge_selection_sets (find_queries_with_label s v.(type) l qs)))) :: execute_selection_set u (filter_queries_with_label l qs);
             
             | _ =>  (l, Leaf Null) :: execute_selection_set u (filter_queries_with_label l qs)
             };
@@ -258,17 +112,19 @@ Section QuerySemantic.
         | None => (l, Leaf Null) :: execute_selection_set u (filter_queries_with_label l qs)
         }
 
-    }.
+    }
+  where "⟦ queries 'in' u ⟧ˢ" := (execute_selection_set u queries).
+  
   all: do ?[by have Hleq := (filter_queries_with_label_leq_size f qs); ssromega].
   all: do ?[by have Hleq := (filter_queries_with_label_leq_size l qs); ssromega].
 
   all: do ?[by rewrite -/(queries_size φ) queries_size_app;
-            have Hleq1 := (found_queries_leq_size v.(type) f qs);
-            have Hleq2 := (merged_selections_leq (find_queries_with_label v.(type) f qs)); ssromega].
+            have Hleq1 := (found_queries_leq_size s v.(type) f qs);
+            have Hleq2 := (merged_selections_leq (find_queries_with_label s v.(type) f qs)); ssromega].
 
   all: do ?[by rewrite -/(queries_size φ) queries_size_app;
-            have Hleq1 := (found_queries_leq_size v.(type) l qs);
-            have Hleq2 := (merged_selections_leq (find_queries_with_label v.(type) l qs)); ssromega].
+            have Hleq1 := (found_queries_leq_size s v.(type) l qs);
+            have Hleq2 := (merged_selections_leq (find_queries_with_label s v.(type) l qs)); ssromega].
 
 
   all: do ? [by rewrite -/(queries_size φ) ?queries_size_app; ssromega].
@@ -302,7 +158,7 @@ Section QuerySemantic.
   
   Lemma exec_preserves_non_existent_label u qs l :
     all (fun q => ~~has_response_name l q) qs ->
-    all (fun kq => kq.1 != l) (execute_selection_set u qs).
+    all (fun kq => kq.1 != l) (⟦ qs in u ⟧ˢ).
   Proof.
     funelim (execute_selection_set u qs) => //=; simp has_response_name => /= /andP [Hne Hall]; do ? apply_andP.
 
@@ -315,7 +171,7 @@ Section QuerySemantic.
 
   
   Lemma exec_responses_are_non_redundant u qs :
-    are_non_redundant (execute_selection_set u qs).
+    Response.are_non_redundant (execute_selection_set u qs).
   Proof.
     apply_funelim (execute_selection_set u qs) => //=; clear u qs => u.
     - move=> f α v qs IH Hv; simp is_non_redundant; rewrite andTb; apply_andP.
@@ -342,7 +198,7 @@ Section QuerySemantic.
       apply: exec_preserves_non_existent_label.
       apply: filtered_queries_hasN_response_name.
 
-    - move=> f ftype α φ qs IH IHqs Hlook; simp is_non_redundant; apply_and3P.
+    - move=> f f' args ftype α φ qs IH IHqs Hlook; simp is_non_redundant. apply_and3P.
       * rewrite all_map; apply/allP => v Hin /=; simp is_non_redundant.
       * apply: exec_preserves_non_existent_label.
         apply: filtered_queries_hasN_response_name.
@@ -351,15 +207,15 @@ Section QuerySemantic.
       apply: exec_preserves_non_existent_label.
       apply: filtered_queries_hasN_response_name.
 
-    - move=> f α v ty φ qs IH IHqs Hv Hlook; simp is_non_redundant; apply_and3P.
+    - move=> f α f' args v ty φ qs IH IHqs Hv Hlook; simp is_non_redundant; apply_and3P.
       apply: exec_preserves_non_existent_label.
       apply: filtered_queries_hasN_response_name.
 
-    - move=> f α ty φ qs IHqs Hv Hlook; simp is_non_redundant; apply_and3P.
+    - move=> f α f' args ty φ qs IHqs Hv Hlook; simp is_non_redundant; apply_and3P.
       apply: exec_preserves_non_existent_label.
       apply: filtered_queries_hasN_response_name.
 
-    - move=> l ftype f α φ qs IH IHqs Hlook; simp is_non_redundant; apply_and3P.
+    - move=> l f' args ftype f α φ qs IH IHqs Hlook; simp is_non_redundant; apply_and3P.
       * rewrite all_map; apply/allP => v Hin /=; simp is_non_redundant.
       * apply: exec_preserves_non_existent_label.
         apply: filtered_queries_hasN_response_name.
@@ -368,17 +224,276 @@ Section QuerySemantic.
       apply: exec_preserves_non_existent_label.
       apply: filtered_queries_hasN_response_name.
 
-    - move=> f α v ty l φ qs IH IHqs Hv Hlook; simp is_non_redundant; apply_and3P.
+    - move=> f α v f' args ty l φ qs IH IHqs Hv Hlook; simp is_non_redundant; apply_and3P.
       apply: exec_preserves_non_existent_label.
       apply: filtered_queries_hasN_response_name.
 
-    - move=> f α ty l φ qs IHqs Hv Hlook; simp is_non_redundant; apply_and3P.
+    - move=> f α f' args ty l φ qs IHqs Hv Hlook; simp is_non_redundant; apply_and3P.
       apply: exec_preserves_non_existent_label.
       apply: filtered_queries_hasN_response_name.
   Qed.
 
+  Reserved Notation "⦃ queries 'in' u ⦄" (at level 50).
   
+   Equations? execute_selection_set2 u (queries : seq (@Query Name Vals)) :
+    seq (Name * ResponseNode) by wf (queries_size queries) :=
+    {
+      execute_selection_set2 _ [::] := [::];
 
+      execute_selection_set2 u (SingleField f α :: qs)
+        with u.(fields) (Field f α) :=
+        {
+        | Some (inl value) => (f, Leaf (SingleValue value)) :: ⦃ qs in u ⦄;
+        | Some (inr values) => (f, Array (map (Leaf \o SingleValue) values)) :: ⦃ qs in u ⦄;
+        | None => (f, Leaf Null) :: ⦃ qs in u ⦄
+        };
+      
+      execute_selection_set2 u (LabeledField l f α :: qs)
+        with u.(fields) (Field f α) :=
+        {
+        | Some (inl value) => (l, Leaf (SingleValue value)) :: ⦃ qs in u ⦄;
+        | Some (inr values) => (l, Array (map (Leaf \o SingleValue) values)) :: ⦃ qs in u ⦄;
+        | None => (l, Leaf Null) :: ⦃ qs in u ⦄
+        };
+
+      
+      execute_selection_set2 u (NestedField f α φ :: qs)
+        with lookup_field_in_type s u.(type) f :=
+        {
+        | Some (Schema.Field _ _ (ListType ty)) => (f, Array [seq Object (⦃ φ in v ⦄) | v <- neighbours_with_field g u (Field f α)]) :: ⦃ qs in u ⦄;
+        
+        | Some (Schema.Field _ _ (NT ty))
+            with ohead (neighbours_with_field g u (Field f α)) :=
+            {
+            | Some v => (f, Object (⦃ φ in v ⦄)) :: ⦃ qs in u ⦄;
+            
+            | _ =>  (f, Leaf Null) :: ⦃ qs in u ⦄
+            };
+
+        | None => (f, Leaf Null) :: ⦃ qs in u ⦄
+        };
+
+       execute_selection_set2 u (NestedLabeledField l f α φ :: qs)
+        with lookup_field_in_type s u.(type) f :=
+        {
+        | Some (Schema.Field _ _ (ListType ty)) => (l, Array [seq Object (⦃ φ in v ⦄) | v <- neighbours_with_field g u (Field f α)]) :: ⦃ qs in u ⦄;
+        
+        | Some (Schema.Field _ _ (NT ty))
+            with ohead (neighbours_with_field g u (Field f α)) :=
+            {
+            | Some v => (l, Object (⦃ φ in v ⦄)) :: ⦃ qs in u ⦄;
+            
+            | _ =>  (l, Leaf Null) :: ⦃ qs in u ⦄
+            };
+
+        | None => (l, Leaf Null) :: ⦃ qs in u ⦄
+        };
+
+       
+        execute_selection_set2 u (InlineFragment t φ :: qs)
+        with does_fragment_type_apply s u.(type) t :=
+        {
+        | true := ⦃ φ ++ qs in u ⦄;
+        | _ := ⦃ qs in u ⦄
+        }
+
+    }
+   where "⦃ queries 'in' u ⦄" := (execute_selection_set2 u queries).
+   all: do ? by ssromega.
+   all: do [by rewrite ?queries_size_app -/(queries_size φ); ssromega].
+  Qed.
+
+ 
+  Lemma filter_queries_with_label_cat l (qs1 qs2 : seq (@Query Name Vals)) :
+    filter_queries_with_label l (qs1 ++ qs2) = filter_queries_with_label l qs1 ++ filter_queries_with_label l qs2.
+  Proof.
+    elim: qs1  => //= hd tl IH.
+    case: hd => //=; intros; simp filter_queries_with_label; do ?[by case: eqP => //= Heq; rewrite IH].
+      by rewrite IH.
+  Qed.
+    
+  Lemma normalize_filter_swap label ty qs :
+    is_object_type s ty ->
+    filter_queries_with_label label (normalize__φ s ty qs) = normalize__φ s ty (filter_queries_with_label label qs).
+  Proof.
+    move=> Hscope.
+    move: {2}(queries_size _) (leqnn (queries_size qs)) => n.
+    elim: n qs => //= [| n IH].
+    - admit.
+    - case=> //; case=> [f α | l f α | f α φ | l f α φ | t φ] qs /= Hleq;
+                            simp normalize; rewrite ?Hscope /=; simp filter_queries_with_label => /=.
+
+    all: do ?[by case: eqP => //= Heq; simp normalize; rewrite Hscope /= IH].
+
+    * case Hlook : lookup_field_in_type => [fld|] //=; rewrite ?Hscope /=; simp filter_queries_with_label => /=.
+      case: eqP => //= Heq; simp normalize.
+      + rewrite IH //; ssromega. 
+      + rewrite Hlook /= Hscope /= IH //; ssromega.
+      + case: eqP => //= Heq; simp normalize; rewrite ?Hlook /= IH //; ssromega.
+
+    * case Hlook : lookup_field_in_type => [fld|] //=; rewrite ?Hscope /=; simp filter_queries_with_label => /=.
+      case: eqP => //= Heq; simp normalize.
+      + rewrite IH //; ssromega. 
+      + rewrite Hlook /= Hscope /= IH //; ssromega.
+      + case: eqP => //= Heq; simp normalize; rewrite ?Hlook /= IH //; ssromega.
+
+
+    * simp normalize; rewrite Hscope /= filter_queries_with_label_cat.
+      rewrite (IH qs) //; do ? ssromega.
+      rewrite (IH φ) //; rewrite -/(queries_size φ) in Hleq; ssromega.
+  Admitted.     
+
+  Lemma lookup_field_return_type ty f fld :
+    lookup_field_in_type s ty f = Some fld ->
+    lookup_field_type s ty f = Some (fld.(return_type)).
+  Admitted.
+
+   
+  Transparent is_field is_inline_fragment qresponse_name qsubqueries.
+
+  Lemma are_similar_fields_share_response_name (q1 q2 : @Query Name Vals) (Hfield1 : q1.(is_field)) (Hfield2 : q2.(is_field)) :
+    are_similar q1 q2 -> (qresponse_name q1 Hfield1) == (qresponse_name q2 Hfield2).
+  Proof.
+    funelim (are_similar q1 q2) => //=.
+  Qed.
+
+   Lemma are_N_similar_fields_N_response_name (q1 q2 : @Query Name Vals) (Hfield1 : q1.(is_field)) (Hfield2 : q2.(is_field)) :
+     ~~are_similar q1 q2 -> (qresponse_name q1 Hfield1) != (qresponse_name q2 Hfield2).
+  Proof.
+    funelim (are_similar q1 q2) => //=.
+  Qed.
+  
+  Lemma filter_not_similar_preserves_list (q : @Query Name Vals) qs (Hfield : q.(is_field)) :
+    all (fun q' => ~~are_similar q' q) qs ->
+    all (fun q' => q'.(is_field)) qs ->
+    filter_queries_with_label (qresponse_name q Hfield) qs = qs.
+  Proof.
+    funelim (filter_queries_with_label _ qs) => //= /andP [Hsim Hall] Hfields; do ? by rewrite H.
+
+    all: do ?[have := (are_N_similar_fields_N_response_name _ q _ Hfield Hsim) => /=-/(_ is_true_true) Hcontr;
+                by rewrite Hcontr in Heq].
+  Qed.
+
+  Lemma find_not_similar_is_nil ty (q : @Query Name Vals) qs (Hfield : q.(is_field)) :
+    all (fun q' => ~~are_similar q' q) qs ->
+    all (fun q' => q'.(is_field)) qs ->
+    find_queries_with_label s ty (qresponse_name q Hfield) qs = [::].
+  Proof.
+  Admitted.
+
+  Lemma asdf qs : all (fun q => q.(is_field)) qs ->
+                  all (is_in_normal_form s) qs ->
+                  are_in_normal_form s qs.
+  Admitted.
+  
+  Theorem execs_on_nrgtnf_are_equivalent u φ :
+    are_in_normal_form s φ ->
+    are_non_redundant φ ->
+    ⦃ φ in u ⦄ = ⟦ φ in u ⟧ˢ.
+  Proof.
+    move: {2}(queries_size _) (leqnn (queries_size φ)) => n.
+    elim: n φ u => [| n IH] φ u.
+    - admit.
+    - case: φ => //=; case=> /= [f α | l f α | f α φ | l f α φ | t φ] qs Hleq.
+      * rewrite /are_in_normal_form /= orbF; simp is_in_normal_form; rewrite andTb => /andP [Hflds Hnf].
+        simp are_non_redundant; rewrite andTb => /=-/andP [Hneq Hnr].
+        simp execute_selection_set; simp execute_selection_set2.
+        case: (u.(fields) _) => //=; [case=> // v|];
+                                 rewrite (filter_not_similar_preserves_list (SingleField f α)) // IH //; by apply: asdf.
+      
+      * rewrite /are_in_normal_form /= orbF; simp is_in_normal_form; rewrite andTb => /andP [Hflds Hnf].
+        simp are_non_redundant; rewrite andTb => /=-/andP [Hneq Hnr].
+        simp execute_selection_set; simp execute_selection_set2.
+        case: (u.(fields) _) => //=; [case=> // v|];
+                                 rewrite (filter_not_similar_preserves_list (LabeledField l f α)) // IH //; by apply: asdf.
+
+        
+      * rewrite /are_in_normal_form /= orbF; simp is_in_normal_form => /and3P [Hfld /andP [Hty Hnf] Hnfs].
+        simp are_non_redundant => /= /and3P [Hsim Hnr Hnrs]. 
+        simp execute_selection_set; simp execute_selection_set2.
+        case Hlook : lookup_field_in_type => [fld|] //=; last rewrite (filter_not_similar_preserves_list (NestedField f α φ)) //.
+        case: fld Hlook => f' args; case=> ty Hlook /=. 
+        + case ohead => //= [v|]; rewrite (filter_not_similar_preserves_list (NestedField f α φ)) //.
+          rewrite (find_not_similar_is_nil v.(type) (NestedField f α φ)) //; simp merge_selection_sets.
+          rewrite cats0 !IH //; admit.
+          rewrite IH //; admit.
+
+        + rewrite (filter_not_similar_preserves_list (NestedField f α φ)) //. 
+          congr cons; [| apply: IH; admit].
+          congr pair; congr Array. apply/eq_in_map => v Hin.
+          rewrite (find_not_similar_is_nil v.(type) (NestedField f α φ)) //; simp merge_selection_sets.
+          rewrite cats0 IH //; admit.
+        + rewrite IH //; admit.
+
+             
+      * rewrite /are_in_normal_form /= orbF; simp is_in_normal_form => /and3P [Hfld /andP [Hty Hnf] Hnfs].
+        simp are_non_redundant => /= /and3P [Hsim Hnr Hnrs]. 
+        simp execute_selection_set; simp execute_selection_set2.
+        case Hlook : lookup_field_in_type => [fld|] //=; last rewrite (filter_not_similar_preserves_list (NestedLabeledField l f α φ)) //.
+        case: fld Hlook => f' args; case=> ty Hlook /=. 
+        + case ohead => //= [v|]; rewrite (filter_not_similar_preserves_list (NestedLabeledField l f α φ)) //.
+          rewrite (find_not_similar_is_nil v.(type) (NestedLabeledField l f α φ)) //; simp merge_selection_sets.
+          rewrite cats0 !IH //; admit.
+          rewrite IH //; admit.
+
+        + rewrite (filter_not_similar_preserves_list (NestedLabeledField l f α φ)) //. 
+          congr cons; [| apply: IH; admit].
+          congr pair; congr Array. apply/eq_in_map => v Hin.
+          rewrite (find_not_similar_is_nil v.(type) (NestedLabeledField l f α φ)) //; simp merge_selection_sets.
+          rewrite cats0 IH //; admit.
+        + rewrite IH //; admit.
+
+
+      * rewrite /are_in_normal_form /=; simp is_in_normal_form => Hnf.
+        simp are_non_redundant => /= /and3P [Hsim Hnr Hnrs].
+        simp execute_selection_set; simp execute_selection_set2.
+        case: does_fragment_type_apply => //=; apply: IH.
+  Admitted.
+
+        
+  
+  Theorem execs_are_equivalent u φ :
+    all (has_valid_fragments s u.(type)) φ ->
+    (⦃ (remove_redundancies s u.(type) (normalize__φ s u.(type) φ)) in u ⦄) = (⟦ φ in u ⟧ˢ).
+  Proof.
+    move: {2}(queries_size _) (leqnn (queries_size φ)) => n.
+    elim: n φ u => /= [| n IH].
+    - admit.
+    - move=> φ u Hleq Hin; have Hscope := (node_in_graph_has_object_type Hin).
+      case: φ Hleq => //.
+      case=> [f α | l f α | f α φ | l f α φ | t φ] qs /= Hleq -/andP [Hv Hvs]; simp normalize;
+              rewrite ?Hscope /=; simp remove_redundancies; simp execute_selection_set.
+
+      * simp execute_selection_set2.
+        case : (u.(fields) _) => //=.
+        + case=> //= v; rewrite normalize_filter_swap // IH //;
+                             do ?[by have Hleq2 := (filter_queries_with_label_leq_size f qs); ssromega].
+          admit.
+          admit.
+        + rewrite normalize_filter_swap // IH //; [by have Hleq2 := (filter_queries_with_label_leq_size f qs); ssromega|].
+          admit.
+      * simp execute_selection_set2.
+        case : (u.(fields) _) => //=.
+        + case=> //= v; rewrite normalize_filter_swap // IH //;
+                             do ?[by have Hleq2 := (filter_queries_with_label_leq_size l qs); ssromega].
+          admit.
+          admit.
+        + rewrite normalize_filter_swap // IH //; [by have Hleq2 := (filter_queries_with_label_leq_size l qs); ssromega|].
+          admit.
+
+      * case Hlook: lookup_field_in_type => [fld|] //=.
+        rewrite Hscope /=; simp remove_redundancies; simp execute_selection_set2.
+        case: fld Hlook => f' args rty Hlook; rewrite Hlook /=.
+        simp execute_selection_set2. rewrite Hlook /=.
+        case: rty Hlook => //= ty Hlook.
+        + case ohead => //= [v|].
+          congr cons; last first.
+          rewrite normalize_filter_swap //.
+          admit.
+          
+          IH //. admit. admit.
+          rewrite normalize_filter_swap // IH.
+   
 
   Equations resolve_field_value u (field_name : Name) (argument_values : {fmap Name -> Vals}) : option ((Vals + seq Vals) + (@node Name Vals) + seq (@node Name Vals)) :=
     {
@@ -457,7 +572,7 @@ Section QuerySemantic.
     - by have Hleq := (filter_queries_with_label_leq_size unknown7 qs); ssromega.
     - by have Hleq := (filter_queries_with_label_leq_size unknown11 qs); ssromega.
   Qed.
-  
+
   
   
   
